proof/proof.ec
@@ -4,50 +4,76 @@ require import Dkc.
 require import Gate.
 require AdvGate.
 
-require import Scheme.
 
-axiom real :
-  forall (Adv <: Scheme.Adv),
-    forall &mDkc,(*forced b to 1 and l to 1*)
-      forall &mGate,
-        Pr[Dkc.Game(Dkc.Dkc, AdvGate.Adv(*(Adv)*)).main()@ &mDkc:res] =
-          Pr[Gate.Game(Scheme.PrvInd, Adv).main()@ &mGate:res].
+lemma real :
+  forall &mDkc,(*forced b to 1 and l to 1*)
+    forall &mGate,
+      forall (Adv <: Gate.Adv),
+        Pr[Dkc.Game(Dkc.Dkc, AdvGate.Adv(Adv)).main()@ &mDkc:res] =
+          Pr[Gate.Game(Gate.PrvInd, Adv).main()@ &mGate:res]
+proof.
+admit.
+save.
 
-axiom middle :
-  forall (Adv <: Scheme.Adv),
-    forall &mDkc1,(*forced b to 0 and l to 1*)
-      forall &mDkc2,(*forced b to 1 and l to 2*)
-        Pr[Dkc.Game(Dkc.Dkc, AdvGate.Adv(*(Adv)*)).main()@ &mDkc1: !res] =
-        Pr[Dkc.Game(Dkc.Dkc, AdvGate.Adv(*(Adv)*)).main()@ &mDkc2:  res].
+lemma middle :
+  forall &mDkc1,(*forced b to 0 and l to 1*)
+    forall &mDkc2,(*forced b to 1 and l to 2*)
+      forall (Adv <: Gate.Adv),
+        Pr[Dkc.Game(Dkc.Dkc, AdvGate.Adv(Adv)).main()@ &mDkc1: !res] =
+        Pr[Dkc.Game(Dkc.Dkc, AdvGate.Adv(Adv)).main()@ &mDkc2:  res]
+proof.
+admit.
+save.
 
-axiom fake :
-  forall (Adv <: Scheme.Adv),
+lemma fake :
+  forall (Adv <: Gate.Adv),
     forall &m,(*forced b to 0 and l to 2*)
-      Pr[Gate.Game(Scheme.PrvInd, Adv).main()@ &m: !res] = 1%r / 2%r.
+      Pr[Dkc.Game(Dkc.Dkc, AdvGate.Adv(Adv)).main()@ &m: !res] = 1%r / 2%r
+proof.
+admit.
+save.
 
-axiom DkcAdv :
+lemma DkcAdv :
   forall (ADVDKC<:Dkc.Adv),
   forall &mDKC,
   forall &mDKC1,(*forced b to 1*)
   forall &mDKC0,(*forced b to 0*)
     2%r * Pr[Dkc.Game(Dkc.Dkc, ADVDKC).main()@ &mDKC:res] - 1%r =
- Pr[Dkc.Game(Dkc.Dkc, ADVDKC).main()@ &mDKC1:res] - Pr[Dkc.Game(Dkc.Dkc, ADVDKC).main()@ &mDKC0: !res].
+ Pr[Dkc.Game(Dkc.Dkc, ADVDKC).main()@ &mDKC1:res] - Pr[Dkc.Game(Dkc.Dkc, ADVDKC).main()@ &mDKC0: !res]
+proof.
+admit.
+save.
 
-axiom DkcGateRelation1 :
+lemma DkcGateRelation1 :
   forall &mDKC,
-    forall (ADVGAR<:Scheme.Adv),
+    forall (Adv<:Gate.Adv),
     forall &mGAR,
-      2%r * Pr[Dkc.Game(Dkc.Dkc, AdvGate.Adv).main()@ &mDKC:res] - 1%r
+      2%r * Pr[Dkc.Game(Dkc.Dkc, AdvGate.Adv(Adv)).main()@ &mDKC:res] - 1%r
         =
-      (2%r * Pr[Gate.Game(Scheme.PrvInd, ADVGAR).main()@ &mGAR:res] - 1%r ) / 6%r.
+      (2%r * Pr[Gate.Game(Gate.PrvInd, Adv).main()@ &mGAR:res] - 1%r ) / 6%r
+proof.
+trivial.
+admit.
+save.
 
-axiom DKCGateRelation2 :
+lemma DKCGateRelation2 :
   forall &mDKC,
-    forall (ADVGAR<:Scheme.Adv),
+    forall (ADVGAR<:Gate.Adv),
     forall &mGAR,
-      Pr[Gate.Game(Scheme.PrvInd, ADVGAR).main()@ &mGAR:res] <= Pr[Dkc.Game(Dkc.Dkc, AdvGate.Adv).main()@ &mDKC:res].
+      Pr[Gate.Game(Gate.PrvInd, ADVGAR).main()@ &mGAR:res] <= Pr[Dkc.Game(Dkc.Dkc, AdvGate.Adv).main()@ &mDKC:res]
+proof.
+admit.
+save.
 
-axiom PrvIndGarble :
+lemma PrvIndGarble :
   forall (epsilon:real),
-    forall (ADV<:Scheme.Adv), forall &m,
-      epsilon > 0%r => Pr[Gate.Game(Scheme.PrvInd, ADV).main()@ &m:res] <= epsilon.
+    forall (ADV<:Gate.Adv), forall &m,
+      epsilon > 0%r => Pr[Gate.Game(Gate.PrvInd, ADV).main()@ &m:res] <= epsilon
+proof.
+intros epsilon ADV &m.
+intros epPos.
+cut trans : (forall (a b c : real), a <= b => b <= c => a <= c).
+trivial.
+apply (trans Pr[Gate.Game(Gate.PrvInd, ADV).main()@ &m:res] Pr[Dkc.Game(Dkc.Dkc, AdvGate.Adv).main()@ &mDKC:res] epsilon _ _).
+admit.
+save.
